working on top level OTP theorem to show off as demo

HMAC/HMAC_specs_equiv.v
@@ -14,59 +14,7 @@ Require Import Cryptol.GetEachN.
 
 Require Import HMAC.HMAC_spec.
 Require Import HMAC.HMAC_lib.
-
-Fixpoint to_bvector (w : nat) (e : ext_val) : option (Bvector w) :=
-  match e,w with
-  | eseq (ebit b :: r),S n =>
-    match to_bvector n (eseq r) with
-    | Some bv => 
-      Some (Vector.cons bool b n bv)
-    | _ => None
-    end
-  | eseq nil, O => Some (Vector.nil bool)
-  | _,_ => None
-  end.
-
-Lemma to_bvector_succeeds :
-  forall l n,
-    has_type (eseq l) (tseq n tbit) ->
-    exists bv,
-      to_bvector n (eseq l) = Some bv.
-Proof.
-  induction l; intros.
-
-  * inversion H. subst. simpl.
-    eauto.
-
-  * inversion H. subst. inversion H2.
-    subst.
-    edestruct IHl. econstructor; eauto.
-    inversion H3. subst.
-    simpl. rewrite H0.
-    eauto.
-Qed.
-
-Lemma bytestream_type :
-  forall l t,
-    Forall (fun x => has_type x t) l ->
-    has_type (eseq l) (tseq (length l) t).
-Proof.
-  induction l; intros.
-  econstructor; eauto.
-  inversion H. subst.
-  econstructor; eauto.
-Qed.
-
-Fixpoint bv_to_extval' {w : nat} (bv : Bvector w) : list ext_val :=
-  match bv with
-  | Vector.nil => nil
-  | Vector.cons b _ r => ebit b :: bv_to_extval' r
-  end.
-  
-Definition bv_to_extval {w : nat} (bv : Bvector w) : ext_val :=
-  let bits := bv_to_extval' bv in
-  let bytes := get_each_n 8 bits in
-  eseq (map eseq bytes).
+Require Import Cryptol.BvectorExt.
 
 (* Bottom out with nil, maybe not a great idea but it's ok *)
 Fixpoint eappend (l : list ext_val) : ext_val :=
