otp/OTP_top.v
@@ -1,0 +1,117 @@
+Require Import Cryptol.Coqlib.
+Require Import Cryptol.BvectorExt.
+Require Import Cryptol.Bitstream.
+Require Import Cryptol.Eager.
+Require Import Cryptol.Semantics.
+Require Import Cryptol.AST.
+
+Require Import otp.FCF.
+Require Import otp.OTP_FCF.
+Require Import otp.OTP_verif.
+Require Import otp.OTP_cryptol.
+
+
+(* cryptol version is otp_encrypt *)
+(* FCF version is OTP_encrypt *)
+
+Lemma same_otp :
+  forall key msg bvkey bvmsg,
+    has_type key byte -> 
+    has_type msg byte ->
+    to_bvector 8%nat key = Some bvkey ->
+    to_bvector 8%nat msg = Some bvmsg ->
+    otp_encrypt key msg = eseq (bv_to_extval' (OTP_encrypt bvkey bvmsg)).
+Proof.
+  intros.
+  inversion H. inversion H0. subst.
+  do 9 (destruct l; try solve [simpl in *; omega]).
+  do 9 (destruct l0; try solve [simpl in *; omega]).
+  clear H. clear H0.
+  repeat match goal with
+         | [ H : Forall _ _ |- _ ] => inversion H; clear H
+         | [ H : has_type ?X tbit |- _ ] => inversion H; subst X; clear H
+         end;
+    subst.
+  simpl in H2. inversion H2. subst.
+  simpl in H1. inversion H1. subst.
+  clear H1 H2.
+  simpl. reflexivity.
+Qed.
+
+Lemma to_bvector_succeeds' :
+  forall v len,
+    has_type v (tseq len tbit) ->
+    exists (bv : Bvector len),
+      to_bvector len v = Some bv.
+Proof.
+  intros. inversion H.
+  subst.
+  eapply to_bvector_succeeds; eauto.
+Qed.
+
+Lemma has_type_xor_ext' :
+  forall len a b,
+    has_type a (tseq len tbit) ->
+    has_type b (tseq len tbit) ->
+    has_type (xor_ext' a b) (tseq len tbit).
+Proof.
+  induction len; intros;
+  inversion H; inversion H0;
+  destruct l; try solve [simpl in *; omega];
+    destruct l0; try solve [simpl in *; omega];
+      subst.
+  simpl. econstructor; eauto.
+  inversion H3. inversion H7.
+  subst x l1 x0 l2.
+  inversion H6. inversion H11.
+  subst e e0.
+  eapply is_seq in H8.
+  eapply is_seq in H12.
+  simpl in H1. simpl in H5. inversion H1. inversion H5.
+  rewrite H9 in *. rewrite H4 in *.
+  eapply (IHlen (eseq l) (eseq l0)) in H8; eauto.
+  clear -H8 H4 H9.
+  inversion H8.
+  destruct (xor_ext l l0) eqn:?; try congruence.
+  inversion H. subst.
+  unfold xor_ext'. unfold xor_ext. fold xor_ext.
+  rewrite Heqo.
+  simpl.
+  replace (S (length l)) with (length (ebit (xorb b b0) :: l2)).
+  econstructor; eauto.
+  econstructor. econstructor; eauto.
+  eauto.
+  simpl. f_equal.
+  assumption.
+Qed.
+
+  
+Theorem cryptol_OTP_secure :
+  forall key msg res bvkey,
+    has_type key byte -> 
+    has_type msg byte ->
+    res = otp_encrypt key msg ->
+    to_bvector 8 key = Some bvkey ->
+    (forall n, @rand_indist 8 (ret bvkey) n) ->
+    eager_eval_expr ge tempty sempty
+                    (EApp (EApp (EVar encrypt) (EValue key)) (EValue msg)) (to_sval res) /\
+    exists bv, to_bvector 8 res = Some bv /\
+               forall n, @rand_indist 8 (ret bv) n.
+Proof.
+  intros.
+  remember H as Hkey. remember H0 as Hmsg.
+  clear HeqHkey. clear HeqHmsg.
+  eapply otp_equiv in H0; try exact H.
+  subst res. split. assumption.
+  assert (has_type (otp_encrypt key msg) byte). {
+
+    unfold otp_encrypt.
+    eapply has_type_xor_ext'; eauto.
+    
+  }
+  eapply to_bvector_succeeds' in H1.
+  destruct H1.
+  exists x. split; auto.
+  intros.
+  (* Just a little needed here *)
+Admitted.
